code/ecdsap256/Hacl.Impl.P256.Ext.fst
@@ -1,0 +1,48 @@
+module Hacl.Impl.P256.Ext
+
+open FStar.HyperStack.All
+open FStar.HyperStack
+open FStar.HyperStack.ST
+
+module ST = FStar.HyperStack.ST
+module HS = FStar.HyperStack
+
+open Lib.IntTypes
+open Lib.Buffer
+
+open Spec.P256.Definitions
+open Hacl.Spec.P256.Felem
+open Spec.P256
+
+open Hacl.Impl.P256.Core
+open Hacl.Impl.P256.Signature.Common
+
+
+open FStar.Mul
+
+
+#set-options "--z3rlimit 150 --max_fuel 0 --max_ifuel 0" 
+
+(** 
+The function takes as input a point as a buffer of uint64.
+It moves the point out of domain, normalises it and writes it down to a uint8 buffer.
+I think. 
+**)
+
+
+val point_to_bin: p: point -> result: lbuffer uint8 (size 64) -> tempBuffer: lbuffer uint64 (size 88) ->
+  Stack uint64 
+  (requires fun h -> live h p /\ live h result /\ live h tempBuffer /\ disjoint tempBuffer p /\ disjoint p result /\
+    point_x_as_nat h p < prime /\
+    point_y_as_nat h p < prime /\
+    point_z_as_nat h p < prime 
+  )
+  (ensures fun h0 _ h1 -> True)
+
+
+let point_to_bin p result tempBuffer = 
+  norm p p tempBuffer;
+  let isPointAtInfinityResult = isPointAtInfinityPrivate p in 
+  pointFromDomain p p;
+  fromFormPoint p result; 
+  isPointAtInfinityResult
